rename Room to Katydid

Validator/Hedge/JSONSchema.lean
@@ -13,7 +13,7 @@ import Validator.Pred.Compare
 
 namespace Hedge
 
-theorem Grammar.Original.decreasing_or_l {α: Type} {σ: Type} [SizeOf σ] (r1 r2: Regex σ) (x: Hedge.Node α):
+theorem Grammar.JSONSchema.decreasing_or_l {α: Type} {σ: Type} [SizeOf σ] (r1 r2: Regex σ) (x: Hedge.Node α):
   Prod.Lex
     (fun a₁ a₂ => sizeOf a₁ < sizeOf a₂)
     (fun a₁ a₂ => sizeOf a₁ < sizeOf a₂)
@@ -22,7 +22,7 @@ theorem Grammar.Original.decreasing_or_l {α: Type} {σ: Type} [SizeOf σ] (r1 r
   apply Prod.Lex.right
   simp +arith only [Regex.or.sizeOf_spec]
 
-theorem Grammar.Original.decreasing_or_r {α: Type} {σ: Type} [SizeOf σ] (r1 r2: Regex σ) (x: Hedge.Node α):
+theorem Grammar.JSONSchema.decreasing_or_r {α: Type} {σ: Type} [SizeOf σ] (r1 r2: Regex σ) (x: Hedge.Node α):
   Prod.Lex
     (fun a₁ a₂ => sizeOf a₁ < sizeOf a₂)
     (fun a₁ a₂ => sizeOf a₁ < sizeOf a₂)
@@ -31,7 +31,7 @@ theorem Grammar.Original.decreasing_or_r {α: Type} {σ: Type} [SizeOf σ] (r1 r
   apply Prod.Lex.right
   simp +arith only [Regex.or.sizeOf_spec]
 
-theorem Grammar.Original.decreasing_concat_l {α: Type} {σ: Type} [SizeOf σ] (r1 r2: Regex σ) (x: Hedge.Node α):
+theorem Grammar.JSONSchema.decreasing_concat_l {α: Type} {σ: Type} [SizeOf σ] (r1 r2: Regex σ) (x: Hedge.Node α):
   Prod.Lex
     (fun a₁ a₂ => sizeOf a₁ < sizeOf a₂)
     (fun a₁ a₂ => sizeOf a₁ < sizeOf a₂)
@@ -40,7 +40,7 @@ theorem Grammar.Original.decreasing_concat_l {α: Type} {σ: Type} [SizeOf σ] (
   apply Prod.Lex.right
   simp +arith only [Regex.concat.sizeOf_spec]
 
-theorem Grammar.Original.decreasing_concat_r {α: Type} {σ: Type} [SizeOf σ] (r1 r2: Regex σ) (x: Hedge.Node α):
+theorem Grammar.JSONSchema.decreasing_concat_r {α: Type} {σ: Type} [SizeOf σ] (r1 r2: Regex σ) (x: Hedge.Node α):
   Prod.Lex
     (fun a₁ a₂ => sizeOf a₁ < sizeOf a₂)
     (fun a₁ a₂ => sizeOf a₁ < sizeOf a₂)
@@ -49,7 +49,7 @@ theorem Grammar.Original.decreasing_concat_r {α: Type} {σ: Type} [SizeOf σ] (
   apply Prod.Lex.right
   simp +arith only [Regex.concat.sizeOf_spec]
 
-theorem Grammar.Original.decreasing_star {α: Type} {σ: Type} [SizeOf σ] (r: Regex σ) (x: Hedge.Node α):
+theorem Grammar.JSONSchema.decreasing_star {α: Type} {σ: Type} [SizeOf σ] (r: Regex σ) (x: Hedge.Node α):
   Prod.Lex
     (fun a₁ a₂ => sizeOf a₁ < sizeOf a₂)
     (fun a₁ a₂ => sizeOf a₁ < sizeOf a₂)
@@ -58,7 +58,7 @@ theorem Grammar.Original.decreasing_star {α: Type} {σ: Type} [SizeOf σ] (r: R
   apply Prod.Lex.right
   simp +arith only [Regex.star.sizeOf_spec]
 
-theorem Grammar.Original.decreasing_symbol {α: Type} {σ: Type} [SizeOf σ] (r1 r2: Regex σ) (label: α) (children: Hedge α) (x: Hedge.Node α) (h: x ∈ children):
+theorem Grammar.JSONSchema.decreasing_symbol {α: Type} {σ: Type} [SizeOf σ] (r1 r2: Regex σ) (label: α) (children: Hedge α) (x: Hedge.Node α) (h: x ∈ children):
   Prod.Lex
     (fun a₁ a₂ => sizeOf a₁ < sizeOf a₂)
     (fun a₁ a₂ => sizeOf a₁ < sizeOf a₂)
@@ -69,7 +69,7 @@ theorem Grammar.Original.decreasing_symbol {α: Type} {σ: Type} [SizeOf σ] (r1
   have h' := List.list_elem_lt h
   omega
 
-theorem Grammar.Original.decreasing_interleave_l {α: Type} {σ: Type} [SizeOf σ] (r1 r2: Regex σ) (x: Hedge.Node α):
+theorem Grammar.JSONSchema.decreasing_interleave_l {α: Type} {σ: Type} [SizeOf σ] (r1 r2: Regex σ) (x: Hedge.Node α):
   Prod.Lex
     (fun a₁ a₂ => sizeOf a₁ < sizeOf a₂)
     (fun a₁ a₂ => sizeOf a₁ < sizeOf a₂)
@@ -78,7 +78,7 @@ theorem Grammar.Original.decreasing_interleave_l {α: Type} {σ: Type} [SizeOf �
   apply Prod.Lex.right
   simp +arith only [Regex.interleave.sizeOf_spec]
 
-theorem Grammar.Original.decreasing_interleave_r {α: Type} {σ: Type} [SizeOf σ] (r1 r2: Regex σ) (x: Hedge.Node α):
+theorem Grammar.JSONSchema.decreasing_interleave_r {α: Type} {σ: Type} [SizeOf σ] (r1 r2: Regex σ) (x: Hedge.Node α):
   Prod.Lex
     (fun a₁ a₂ => sizeOf a₁ < sizeOf a₂)
     (fun a₁ a₂ => sizeOf a₁ < sizeOf a₂)
@@ -87,7 +87,7 @@ theorem Grammar.Original.decreasing_interleave_r {α: Type} {σ: Type} [SizeOf �
   apply Prod.Lex.right
   simp +arith only [Regex.interleave.sizeOf_spec]
 
-theorem Grammar.Original.decreasing_and_l {α: Type} {σ: Type} [SizeOf σ] (r1 r2: Regex σ) (x: Hedge.Node α):
+theorem Grammar.JSONSchema.decreasing_and_l {α: Type} {σ: Type} [SizeOf σ] (r1 r2: Regex σ) (x: Hedge.Node α):
   Prod.Lex
     (fun a₁ a₂ => sizeOf a₁ < sizeOf a₂)
     (fun a₁ a₂ => sizeOf a₁ < sizeOf a₂)
@@ -96,7 +96,7 @@ theorem Grammar.Original.decreasing_and_l {α: Type} {σ: Type} [SizeOf σ] (r1 
   apply Prod.Lex.right
   simp +arith only [Regex.and.sizeOf_spec]
 
-theorem Grammar.Original.decreasing_and_r {α: Type} {σ: Type} [SizeOf σ] (r1 r2: Regex σ) (x: Hedge.Node α):
+theorem Grammar.JSONSchema.decreasing_and_r {α: Type} {σ: Type} [SizeOf σ] (r1 r2: Regex σ) (x: Hedge.Node α):
   Prod.Lex
     (fun a₁ a₂ => sizeOf a₁ < sizeOf a₂)
     (fun a₁ a₂ => sizeOf a₁ < sizeOf a₂)
@@ -105,7 +105,7 @@ theorem Grammar.Original.decreasing_and_r {α: Type} {σ: Type} [SizeOf σ] (r1 
   apply Prod.Lex.right
   simp +arith only [Regex.and.sizeOf_spec]
 
-theorem Grammar.Original.decreasing_compliment {α: Type} {σ: Type} [SizeOf σ] (r1: Regex σ) (x: Hedge.Node α):
+theorem Grammar.JSONSchema.decreasing_compliment {α: Type} {σ: Type} [SizeOf σ] (r1: Regex σ) (x: Hedge.Node α):
   Prod.Lex
     (fun a₁ a₂ => sizeOf a₁ < sizeOf a₂)
     (fun a₁ a₂ => sizeOf a₁ < sizeOf a₂)
@@ -114,7 +114,7 @@ theorem Grammar.Original.decreasing_compliment {α: Type} {σ: Type} [SizeOf σ]
   apply Prod.Lex.right
   simp +arith only [Regex.compliment.sizeOf_spec]
 
-def Grammar.Original.derive (G: Grammar n φ) (Φ: φ → α → Bool)
+def Grammar.JSONSchema.derive (G: Grammar n φ) (Φ: φ → α → Bool)
   (r: Regex (φ × Ref n)) (node: Node α): Regex (φ × Ref n) :=
   match r with
   | Regex.emptyset => Regex.emptyset
@@ -167,7 +167,7 @@ def Grammar.Original.derive (G: Grammar n φ) (Φ: φ → α → Bool)
     · apply decreasing_and_r
     · apply decreasing_compliment
 
-namespace Grammar.Original
+namespace Grammar.JSONSchema
 
 def validate (G: Grammar n φ) (Φ: φ → α → Bool)
   (nodes: Hedge α): Bool :=
@@ -176,13 +176,13 @@ def filter (G: Grammar n φ) (Φ: φ → α → Bool)
   (hedges: List (Hedge α)): List (Hedge α) :=
     List.filter (validate G Φ) hedges
 
-end Grammar.Original
+end Grammar.JSONSchema
 
-theorem Grammar.Original.derive_commutes (G: Grammar n φ) Φ [DecidableRel Φ]
+theorem Grammar.JSONSchema.derive_commutes (G: Grammar n φ) Φ [DecidableRel Φ]
   (r: Regex (φ × Ref n)) (node: Node α):
-  Rule.denote G Φ (Grammar.Original.derive G (decideRel Φ) r node)
+  Rule.denote G Φ (Grammar.JSONSchema.derive G (decideRel Φ) r node)
   = Lang.derive (Rule.denote G Φ r) node := by
-  fun_induction (Grammar.Original.derive G (fun p a => Φ p a)) r node with
+  fun_induction (Grammar.JSONSchema.derive G (fun p a => Φ p a)) r node with
   | case1 => -- emptyset
     rw [Hedge.Grammar.denote_emptyset]
     rw [Lang.derive_emptyset]
@@ -264,20 +264,20 @@ theorem Grammar.Original.derive_commutes (G: Grammar n φ) Φ [DecidableRel Φ]
     unfold Lang.compliment
     rfl
 
-theorem Grammar.Original.derives_commutes (G: Hedge.Grammar n φ) (Φ: φ → α → Prop) [DecidableRel Φ] (r: Regex (φ × Ref n)) (nodes: Hedge α):
-  Hedge.Grammar.Rule.denote G Φ (List.foldl (Grammar.Original.derive G (decideRel Φ)) r nodes) = Lang.derives (Hedge.Grammar.Rule.denote G Φ r) nodes := by
+theorem Grammar.JSONSchema.derives_commutes (G: Hedge.Grammar n φ) (Φ: φ → α → Prop) [DecidableRel Φ] (r: Regex (φ × Ref n)) (nodes: Hedge α):
+  Hedge.Grammar.Rule.denote G Φ (List.foldl (Grammar.JSONSchema.derive G (decideRel Φ)) r nodes) = Lang.derives (Hedge.Grammar.Rule.denote G Φ r) nodes := by
   rw [Lang.derives_foldl]
   induction nodes generalizing r with
   | nil =>
     simp only [List.foldl_nil]
   | cons x xs ih =>
     simp only [List.foldl_cons]
-    have h := Grammar.Original.derive_commutes G Φ r x
-    have ih' := ih (Grammar.Original.derive G (decideRel Φ) r x)
+    have h := Grammar.JSONSchema.derive_commutes G Φ r x
+    have ih' := ih (Grammar.JSONSchema.derive G (decideRel Φ) r x)
     rw [h] at ih'
     exact ih'
 
-theorem Grammar.Original.validate_commutes (G: Hedge.Grammar n φ) (Φ: φ → α → Prop) [DecidableRel Φ] (nodes: Hedge α):
+theorem Grammar.JSONSchema.validate_commutes (G: Hedge.Grammar n φ) (Φ: φ → α → Prop) [DecidableRel Φ] (nodes: Hedge α):
   (validate G (decideRel Φ) nodes = true) = (Hedge.Grammar.denote G Φ) nodes := by
   unfold Hedge.Grammar.denote
   rw [<- Lang.validate (Hedge.Grammar.Rule.denote G Φ G.start) nodes]
@@ -287,7 +287,7 @@ theorem Grammar.Original.validate_commutes (G: Hedge.Grammar n φ) (Φ: φ → �
 
 -- Tests
 
-namespace Grammar.Original
+namespace Grammar.JSONSchema
 
 open Pred
 
