Validator/Regex/IfExpr.lean
@@ -1,3 +1,3 @@
 import Validator.Regex.IfExpr.Enter
 import Validator.Regex.IfExpr.IfExpr
-import Validator.Regex.IfExpr.Room
+import Validator.Regex.IfExpr.Katydid
